\subsection{Informal derivation of Xiang's approach}
Consider the stochastic dynamics $(d=1)$:
$$
X^{n+1}=X^n-\eta\left( HX^n+\sqrt{\Sigma}Z^{n} \right) ,Z^{n}\sim N(0,I)
$$
so, $X^n$ remains Gaussian.
\begin{equation*}
    \begin{aligned}
        &X^{n+1}=\left(1-\eta H\right) X^n-\eta \sqrt{\Sigma}Z^{n} \\
        \Rightarrow& \frac{X^{n+1}}{\left(1-\eta H\right)^{n+1}} = \frac{X^{n}}{\left(1-\eta H\right)^{n}}-\frac{\eta \sqrt{\Sigma}Z^{n}}{\left(1-\eta H\right)^{n+1}}\\
        \Rightarrow& \frac{X^{n}}{\left(1-\eta H\right)^{n}} =X^0 - \eta\sqrt{\Sigma}\sum_{i = 1}^{n}\frac{Z^i}{\left(1-\eta H\right)^{i}} \\
        \Rightarrow& X^{n} =\left(1-\eta H\right)^{n}X^0 -\eta\sqrt{\Sigma}\sum_{i = 1}^{n}\left(1-\eta H\right)^{n-i}Z^i
    \end{aligned}
\end{equation*}
We can further calculate its mean and variance:
$$
m^n = \mathbb{E} X^n = (1-\eta H)^n \mathbb{E} X^0
$$
\begin{equation*}
    \begin{aligned}
        \mathbb{E}\left[ (x^n-m^n)(x^n-m^n)^T \right] =& \eta^2\Sigma  \sum_{i = 1}^{n}(1-\eta H)^{2(n-i)}\\
        =&\eta^2\Sigma \sum_{i = 0}^{n-1}(1-\eta H)^{2i}\\
        =&\eta^2\Sigma\frac{1-(1-\eta H)^{2n}}{1-(1-\eta H)^2}
    \end{aligned}
\end{equation*}
Following the idea of principle flow, first we let the mean of two meet:
\begin{equation*}
    \begin{aligned}
        &(1-\eta H)^n = \exp(Fn\eta)\\
        \Rightarrow& F = \log(1-\eta H)/\eta
    \end{aligned}
\end{equation*}
then look at the variance:
$$
\int_{0}^{t} \exp(F(t-\tau))\widehat{\Sigma}\exp(F(t-\tau))^T \,d\tau = \eta^2\Sigma\frac{1-(1-\eta H)^{2n}}{2\eta H-(\eta H)^2}
$$
For the left side, we have:
\begin{equation*}
    \begin{aligned}
        \int_{0}^{t} \exp(F(t-\tau))\widehat{\Sigma}\exp(F(t-\tau))^T \,d\tau &= \frac{1}{2F}\exp(2F\tau)\mid _0^{t}\widehat{\Sigma}\\
        &=\frac{1}{2F}\widehat{\Sigma}\cdot(\exp(2Fn\eta)-1)\\
        &=\frac{(1-\eta H)^{2n}-1}{2F}\cdot\widehat{\Sigma}
    \end{aligned}
\end{equation*}
So,
\begin{equation*}
    \begin{aligned}
        &\frac{(1-\eta H)^{2n}-1}{2F}\cdot\widehat{\Sigma} =  \eta^2\Sigma\frac{1-(1-\eta H)^{2n}}{2\eta H-(\eta H)^2}\\
        \Rightarrow& \widehat{\Sigma} = -\frac{2F\cdot\eta^2\cdot\Sigma}{2\eta H - \eta^2H^2} = \frac{2\Sigma\log(1-\eta H)}{H(H\eta-2)}
    \end{aligned}
\end{equation*}









